compiler/backend/proofs/bvl_constProofScript.sml
@@ -2,100 +2,206 @@ open preamble bvl_constTheory bvlSemTheory bvlPropsTheory;
 
 val _ = new_theory"bvl_constProof";
 
-val ind = evaluate_ind
-  |> Q.SPECL [`\(xs,env,s). (FST (evaluate (xs,env,s)) <> Rerr(Rabort Rtype_error)) ==>
-                            evaluate (compile_exps xs,env,s) = evaluate (xs,env,s)`]
-  |> SIMP_RULE std_ss []
+val v_rel_def = Define `
+  v_rel (:'a) a x y xs ys =
+    case a of
+    | Var n => LLOOKUP ys n = SOME x
+    | Op _ _ => !(s:'a bvlSem$state) env. evaluate ([a],env,s) = (Rval [x],s)
+    | _ => F`;
 
-val bEval_cons = evaluate_CONS;
-val bEval_def = evaluate_def;
-val bEvalOp_def = do_app_def;
+val env_rel_def = Define `
+  (env_rel (:'a) [] e1 e2 = (e1 = e2)) /\
+  (env_rel (:'a) (NONE::rest) (x::e1) (y::e2) <=>
+     (x = y) /\ env_rel (:'a) rest e1 e2) /\
+  (env_rel (:'a) (SOME a::rest) (x::e1) (y::e2) <=>
+     v_rel (:'a) a x y (x::e1) (y::e2) /\ env_rel (:'a) rest e1 e2) /\
+  (env_rel _ _ _ _ = F)`
 
-val compile_exps_thm = store_thm("compile_exps_thm",
-  ``!xs env s.
-      (FST (evaluate (xs,env,s)) <> Rerr(Rabort Rtype_error)) ==>
-      (evaluate (compile_exps xs,env,s) = evaluate (xs,env,s))``,
-  HO_MATCH_MP_TAC ind \\ REPEAT STRIP_TAC
-  \\ SIMP_TAC std_ss [compile_exps_def,LET_DEF]
-  \\ POP_ASSUM MP_TAC
+val env_rel_length = store_thm("env_rel_length",
+  ``!ax env env2. env_rel (:α) ax env env2 ==> LENGTH env2 = LENGTH env``,
+  Induct \\ Cases_on `env` \\ Cases_on `env2` \\ fs [env_rel_def]
+  \\ Cases \\ fs [env_rel_def]);
+
+val env_rel_LLOOKUP_NONE = prove(
+  ``!ax env env2 n.
+      env_rel (:α) ax env env2 /\
+      (LLOOKUP ax n = NONE \/ LLOOKUP ax n = SOME NONE) ==>
+      EL n env2 = EL n env``,
+  Induct \\ Cases_on `env` \\ Cases_on `env2` \\ fs [env_rel_def]
+  \\ Cases \\ fs [env_rel_def,LLOOKUP_def]
+  \\ rw [] \\ fs [] \\ Cases_on `n` \\ fs [EL]);
+
+val env_rel_LOOKUP_SOME = prove(
+  ``!env env2 ax x n.
+      env_rel (:α) ax env env2 /\
+      LLOOKUP ax n = SOME (SOME x) ==>
+      v_rel (:'a) x (EL n env) (EL n env2) (DROP n env) (DROP n env2)``,
+  Induct \\ Cases_on `env2` \\ Cases_on `ax` \\ fs [env_rel_def,LLOOKUP_def]
+  \\ rw [] \\ fs [env_rel_def] \\ res_tac \\ fs []
+  \\ Cases_on `n` \\ fs [env_rel_def]
+  \\ first_x_assum match_mp_tac
+  \\ Cases_on `h'` \\ fs [env_rel_def]);
+
+val evaluate_delete_var_Rerr_SING = store_thm("evaluate_delete_var_Rerr_SING",
+  ``!x s r e env2.
+      evaluate ([x],env2,s) = (Rerr e,r) /\
+      e <> Rabort Rtype_error ==>
+      evaluate ([bvl_const$delete_var x],env2,s) = (Rerr e,r)``,
+  Cases \\ fs [delete_var_def]
+  \\ fs [evaluate_def,do_app_def] \\ rw []
+  \\ CCONTR_TAC \\ fs [] \\ rw []);
+
+val evaluate_delete_var_Rerr = prove(
+  ``!xs s r e env2.
+      evaluate (xs,env2,s) = (Rerr e,r) /\
+      e <> Rabort Rtype_error ==>
+      evaluate (MAP bvl_const$delete_var xs,env2,s) = (Rerr e,r)``,
+  Induct \\ fs [] \\ once_rewrite_tac [evaluate_CONS]
+  \\ rw [] \\ every_case_tac \\ fs [] \\ rw []
+  \\ TRY (drule evaluate_delete_var_Rerr_SING \\ fs [])
+  \\ res_tac \\ fs []
+  \\ Cases_on `h` \\ fs [delete_var_def]
+  \\ rw [] \\ fs []
+  \\ fs [evaluate_def,do_app_def] \\ rw []
+  \\ every_case_tac \\ fs [] \\ rw []);
+
+val evaluate_delete_var_Rval = prove(
+  ``!xs env2 s a r ax env.
+      evaluate (xs,env2,s:'a bvlSem$state) = (Rval a,r) /\
+      env_rel (:'a) ax env env2 ==>
+      ?b. evaluate (MAP delete_var xs,env2,s) = (Rval b,r) /\
+          env_rel (:'a) (extract_list xs ++ ax) (a ++ env) (b ++ env2)``,
+  Induct \\ fs [env_rel_def,extract_list_def]
+  \\ once_rewrite_tac [evaluate_CONS]
+  \\ rw [] \\ Cases_on `evaluate ([h],env2,s)` \\ fs []
+  THEN1 (imp_res_tac evaluate_IMP_LENGTH \\ Cases_on `a` \\ fs [])
+  \\ Cases_on `q` \\ fs []
+  \\ Cases_on `?i. h = Var i` \\ fs []
   THEN1
-   (SIMP_TAC std_ss [Once bEval_cons]
-    \\ ONCE_REWRITE_TAC [EQ_SYM_EQ]
-    \\ SIMP_TAC std_ss [Once bEval_cons]
-    \\ FULL_SIMP_TAC std_ss [compile_exp_SING]
-    \\ BasicProvers.EVERY_CASE_TAC
-    \\ FULL_SIMP_TAC (srw_ss()) [compile_exps_def,bEval_def]
-    \\ REV_FULL_SIMP_TAC (srw_ss()) [compile_exps_def])
+   (rw [] \\ fs [delete_var_def,evaluate_def,do_app_def]
+    \\ every_case_tac \\ fs [] \\ rw []
+    \\ res_tac \\ fs [extract_def,env_rel_def] \\ rw []
+    \\ fs [v_rel_def,LLOOKUP_EQ_EL]
+    \\ imp_res_tac evaluate_IMP_LENGTH \\ fs []
+    \\ fs [GSYM ADD1,ADD_CLAUSES,EL_APPEND2])
+  \\ `delete_var h = h` by (Cases_on `h` \\ fs [delete_var_def]) \\ fs []
+  \\ Cases_on `evaluate (xs,env2,r')` \\ fs [] \\ Cases_on `q` \\ fs []
+  \\ res_tac \\ fs [] \\ rw []
+  \\ Cases_on `extract h xs` \\ fs [env_rel_def]
+  \\ imp_res_tac evaluate_SING \\ rw [] \\ fs []
+  \\ Cases_on `h` \\ fs [extract_def]
+  \\ rename1 `bvl_const$extract (Op opp ll) _ = SOME xx`
+  \\ Cases_on `opp` \\ fs [extract_def] \\ rw []
+  \\ every_case_tac \\ fs []
+  \\ fs [v_rel_def,LENGTH_NIL,evaluate_def,do_app_def]
+  \\ every_case_tac \\ fs []);
+
+val IS_SOME_dest_Op_Const = store_thm("IS_SOME_dest_Op_Const[simp]",
+  ``IS_SOME (dest_Op_Const h) = ?i. h = Op (Const i) []``,
+  Cases_on `h` \\ fs [dest_Op_Const_def]
+  \\ Cases_on `o'` \\ fs [dest_Op_Const_def]
+  \\ rw [] \\ fs [LENGTH_NIL]);
+
+val evaluate_EQ_NIL = store_thm("evaluate_EQ_NIL",
+  ``bvlSem$evaluate (xs,env,s) = (Rval [],t) <=> xs = [] /\ s = t``,
+  mp_tac (Q.SPECL [`xs`,`env`,`s`] evaluate_LENGTH)
+  \\ every_case_tac \\ fs []
+  \\ rw [] \\ TRY eq_tac \\ fs [] \\ rw [] \\ fs [LENGTH_NIL]
+  \\ CCONTR_TAC \\ fs [] \\ fs [evaluate_def]);
+
+val is_simple_thm = store_thm("is_simple_thm",
+  ``is_simple v <=> (?t. v = Op (Cons t) []) \/ (?i. v = Op (Const i) [])``,
+  Cases_on `v` \\ fs [is_simple_def]
+  \\ Cases_on `o'` \\ fs [is_simple_def,LENGTH_NIL]);
+
+val SmartOp_thm = store_thm("SmartOp_thm",
+  ``evaluate ([Op op xs],env,s) = (res,s2) /\
+    res ≠ Rerr (Rabort Rtype_error) ==>
+    evaluate ([SmartOp op xs],env,s) = (res,s2)``,
+  full_simp_tac std_ss [SmartOp_def]
+  \\ reverse (Cases_on `op`) \\ fs [] \\ every_case_tac \\ fs []
+  \\ fs [quantHeuristicsTheory.LIST_LENGTH_7] \\ rw []
+  \\ fs [dest_Op_Const_def,evaluate_def,do_app_def] \\ rw []
+  \\ fs [dest_Op_Const_def,evaluate_def,do_app_def] \\ rw []
+  \\ rfs [] \\ fs [is_simple_thm] \\ rfs [] \\ rw []
+  \\ fs [dest_Op_Const_def,evaluate_def,do_app_def] \\ rw []
+  \\ eq_tac \\ rw []);
+
+val evaluate_env_rel = store_thm("evaluate_env_rel",
+  ``!xs env1 (s1:'a bvlSem$state) ax env2 res s2 ys.
+      (evaluate (xs,env1,s1) = (res,s2)) /\
+      env_rel (:'a) ax env1 env2 /\
+      res <> Rerr (Rabort Rtype_error) ==>
+      (evaluate (compile ax xs,env2,s1) = (res,s2))``,
+  recInduct evaluate_ind \\ REPEAT STRIP_TAC
+  \\ FULL_SIMP_TAC std_ss [compile_def,evaluate_def,compile_HD_SING]
   THEN1
-   (SRW_TAC [] [] \\ POP_ASSUM MP_TAC \\ fs [bEval_def]
-    \\ Cases_on `evaluate ([x1],env,s)` \\ fs []
-    \\ reverse (Cases_on `q`) \\ fs []
-    \\ fs [GSYM compile_exp_SING,EVAL ``Bool T``,EVAL ``Bool F``]
-    \\ fs [bEval_def,bEvalOp_def] \\ SRW_TAC [] []
-    \\ fs [EVAL ``Boolv T``,EVAL ``Boolv F``])
-  \\ TRY
-   (ASM_SIMP_TAC std_ss [bEval_def]
-    \\ BasicProvers.EVERY_CASE_TAC
-    \\ FULL_SIMP_TAC (srw_ss()) [GSYM compile_exp_SING]
-    \\ REV_FULL_SIMP_TAC (srw_ss()) [] \\ NO_TAC)
-  \\ SIMP_TAC std_ss [bEval_def,compile_op_def]
-  \\ reverse (Cases_on `EVERY isConst (compile_exps xs)`)
-  THEN1 (FULL_SIMP_TAC std_ss [bEval_def]
-         \\ Cases_on `evaluate (xs,env,s)` \\ FULL_SIMP_TAC (srw_ss()) []
-         \\ Cases_on `q` \\ FULL_SIMP_TAC (srw_ss()) [])
-  \\ Cases_on `?s1. evaluate (xs,env,s) = (Rerr(Rabort Rtype_error),s1)` \\ fs [LET_DEF]
-  \\ Cases_on `evaluate (xs,env,s)` \\ fs []
-  \\ IMP_RES_TAC evaluate_isConst
-  \\ FULL_SIMP_TAC std_ss []
-  \\ SRW_TAC [] []
-  \\ Cases_on `op` \\ FULL_SIMP_TAC (srw_ss()) [bEval_def]
-  \\ Cases_on `xs` \\ fs [compile_exps_def,bEvalOp_def]
-  \\ Cases_on `t` \\ fs [compile_exps_def,bEvalOp_def]
-  \\ `t' = []` by ALL_TAC \\ fs [compile_exps_def] \\ SRW_TAC [] [] \\ fs []
-  \\ Cases_on `REVERSE (MAP (Number o getConst) (compile_exps t'))` \\ fs []
-  \\ TRY (Cases_on `t'` \\ fs [compile_exps_def] \\ NO_TAC)
-  \\ TRY (simp[Boolv_def] \\ NO_TAC)
-  \\ Cases_on `h''` \\ fs []
-  \\ Cases_on `t` \\ fs []
-  \\ Cases_on `h''` \\ fs []
-  \\ Cases_on `t''` \\ fs []);
+   (`?y0. compile ax [x] = [y0]` by
+     (`LENGTH (compile ax [x]) = LENGTH [x]` by fs [compile_length]
+      \\ Cases_on `compile ax [x]` \\ fs [LENGTH_NIL])
+    \\ `?y1 ys. compile ax (y::xs) = y1::ys` by
+     (`LENGTH (compile ax (y::xs)) = LENGTH (y::xs)` by fs [compile_length]
+      \\ Cases_on `compile ax (y::xs)` \\ fs [LENGTH_NIL])
+    \\ fs [] \\ every_case_tac \\ fs [] \\ rw [] \\ fs []
+    \\ rpt (first_x_assum drule) \\ fs []
+    \\ rw [] \\ rpt (first_x_assum drule) \\ fs [] \\ rw []
+    \\ fs [evaluate_def])
+  THEN1
+   (Cases_on `n < LENGTH env` \\ fs [] \\ rw []
+    \\ Cases_on `LLOOKUP ax n` \\ fs []
+    \\ imp_res_tac env_rel_length
+    THEN1 (fs [evaluate_def] \\ metis_tac [env_rel_LLOOKUP_NONE])
+    \\ CASE_TAC
+    THEN1 (fs [evaluate_def] \\ metis_tac [env_rel_LLOOKUP_NONE])
+    \\ CASE_TAC
+    \\ drule env_rel_LOOKUP_SOME \\ fs [] \\ fs [v_rel_def]
+    \\ disch_then drule \\ fs [] \\ rw []
+    \\ fs [evaluate_def]
+    \\ fs [LLOOKUP_EQ_EL]
+    \\ fs [EL_DROP] \\ rfs [EL_DROP])
+  THEN1
+   (Cases_on `evaluate ([x1],env,s)` \\ fs []
+    \\ Cases_on `q` \\ fs [] \\ rw [] \\ res_tac \\ fs []
+    \\ every_case_tac \\ fs []
+    \\ imp_res_tac evaluate_SING \\ fs [] \\ rveq \\ fs []
+    \\ res_tac \\ fs []
+    \\ fs [evaluate_def,compile_HD_SING]
+    \\ imp_res_tac (prove(``x = y ==> [x] = [y]``,fs []))
+    \\ full_simp_tac std_ss [compile_HD_SING]
+    \\ fs [evaluate_def,EVAL ``Bool T``,EVAL ``Bool F``])
+  THEN1
+   (fs [LET_THM,evaluate_def]
+    \\ Cases_on `evaluate (xs,env,s)` \\ fs []
+    \\ Cases_on `q` \\ fs [] \\ rw []
+    \\ res_tac \\ fs []
+    \\ imp_res_tac evaluate_delete_var_Rerr \\ fs []
+    \\ drule evaluate_delete_var_Rval \\ fs [compile_HD_SING]
+    \\ disch_then drule \\ strip_tac \\ fs [])
+  THEN1
+   (Cases_on `evaluate ([x1],env,s)` \\ fs []
+    \\ Cases_on `q` \\ fs [] \\ rw [] \\ res_tac \\ fs []
+    \\ every_case_tac \\ fs [])
+  THEN1
+   (Cases_on `evaluate ([x1],env,s1)` \\ fs [] \\ Cases_on `q` \\ fs []
+    \\ res_tac \\ rw [] \\ Cases_on `e` \\ fs [] \\ rw [] \\ fs []
+    \\ first_x_assum match_mp_tac
+    \\ fs [env_rel_def])
+  \\ TRY (match_mp_tac SmartOp_thm)
+  \\ fs [evaluate_def] \\ every_case_tac \\ fs [] \\ rw [] \\ fs []
+  \\ res_tac \\ fs [] \\ rw [] \\ fs [] \\ rw [] \\ fs []);
 
-(* these theorems are unnecessary, since bvl_handle happens after bvl_const
-val compile_exps_bVarBound = Q.store_thm("compile_exps_bVarBound",
-  `(∀es n. bVarBound n es ⇒ bVarBound n (compile_exps es)) ∧
-   (∀e n. bVarBound n [e] ⇒ bVarBound n [compile_exp e])`,
-  ho_match_mp_tac compile_exps_ind >>
-  rw[compile_exps_def] >> rw[] >> fs[] >> rfs[] >>
-  fs[bVarBound_def,clos_to_bvlTheory.Bool_def] >>
-  TRY (
-    CHANGED_TAC(rw[compile_op_def]) >>
-    BasicProvers.CASE_TAC >> rw[] ) >>
-  fs[Once bVarBound_EVERY] >>
-  METIS_TAC[bVarBound_EVERY]);
+val compile_thm = save_thm("compile_thm",
+  evaluate_env_rel
+  |> Q.SPECL [`xs`,`env`,`s1`,`[]`,`env`] |> GEN_ALL
+  |> SIMP_RULE std_ss [env_rel_def])
 
-val compile_exps_isVar = Q.store_thm("compile_exps_isVar",
-  `(∀es. EVERY isVar es ⇒ EVERY isVar (compile_exps es)) ∧
-   (∀e. isVar e ⇒ isVar (compile_exp e))`,
-  ho_match_mp_tac compile_exps_ind >>
-  rw[compile_exps_def,isVar_def]);
-
-val compile_exps_GoodHandleLet = Q.store_thm("compile_exps_GoodHandleLet",
-  `(∀es.  bEvery GoodHandleLet es ⇒ bEvery GoodHandleLet (compile_exps es)) ∧
-   (∀e. bEvery GoodHandleLet [e] ⇒ bEvery GoodHandleLet [compile_exp e])`,
-  ho_match_mp_tac compile_exps_ind >>
-  rw[compile_exps_def] >> rw[] >> fs[] >>
-  TRY (
-    CHANGED_TAC(rw[compile_op_def]) >>
-    BasicProvers.CASE_TAC >> rw[] ) >>
-  TRY (
-    qmatch_assum_rename_tac`GoodHandleLet (Handle e1 e2)` >>
-    Cases_on`e1`>>fs[compile_exps_def] >>
-    imp_res_tac compile_exps_bVarBound >>
-    imp_res_tac compile_exps_isVar >>
-    imp_res_tac compile_exps_bVarBound >>
-    fs[compile_exps_SING] ) >>
-  fs[Once bEvery_EVERY] >>
-  METIS_TAC[bEvery_EVERY]);
-*)
+val evaluate_compile_exp = store_thm("evaluate_compile_exp",
+  ``evaluate ([d],env,s) = (r,t) /\
+    r <> Rerr (Rabort Rtype_error) ==>
+    evaluate ([bvl_const$compile_exp d],env,s) = (r,t)``,
+  fs [compile_exp_def]
+  \\ `LENGTH (compile [] [d]) = LENGTH [d]` by fs [compile_length]
+  \\ Cases_on `compile [] [d]` \\ fs [LENGTH_NIL] \\ rw []
+  \\ imp_res_tac compile_thm \\ rfs []);
 
 val _ = export_theory();
