compiler/backend/proofs/bvl_handleProofScript.sml
@@ -1,73 +1,282 @@
 open preamble bvl_handleTheory bvlSemTheory bvlPropsTheory;
+open indexedListsTheory;
 
 val _ = new_theory"bvl_handleProof";
 
-val evaluate_GENLIST =
+(* TODO: move *)
+
+val MAPi_ID = store_thm("MAPi_ID[simp]",
+  ``MAPi (\x y. y) = I``,
+  fs [FUN_EQ_THM] \\ Induct \\ fs [o_DEF]);
+
+(* -- *)
+
+val no_raise_evaluate = store_thm("no_raise_evaluate",
+  ``!xs env s1 res r.
+      no_raise xs /\ (evaluate (xs,env,s1) = (res,r)) ==>
+      !a. res <> Rerr (Rraise a)``,
+  recInduct evaluate_ind \\ REPEAT STRIP_TAC \\ rw []
+  \\ pop_assum mp_tac \\ fs []
+  \\ once_rewrite_tac [evaluate_def] \\ fs [no_raise_def]
+  \\ every_case_tac \\ fs [] \\ res_tac \\ fs []
+  \\ CCONTR_TAC \\ rw [] \\ fs [] \\ rveq
+  \\ imp_res_tac do_app_err \\ fs []);
+
+val evaluate_GENLIST = save_thm("evaluate_GENLIST",
   evaluate_genlist_vars
   |> Q.SPECL[`0`,`env ++ ys`,`LENGTH (env:bvlSem$v list)`,`s`]
-  |> SIMP_RULE(srw_ss()++ETA_ss)[TAKE_APPEND1];
+  |> SIMP_RULE(srw_ss()++ETA_ss)[TAKE_APPEND1]);
 
-val compile_correct = Q.prove(
-  `!xs env s1 res s2 ys.
-     (evaluate (xs,env,s1) = (res,s2)) /\ res <> Rerr(Rabort Rtype_error) ==>
-     (evaluate (compile (LENGTH env) xs,env ++ ys,s1) = (res,s2))`,
+val env_rel_def = Define `
+  env_rel l env env1 =
+    LIST_RELi (\i v1 v2. has_var i l ==> v1 = v2) env env1`
+
+val env_rel_mk_Union = store_thm("env_rel_mk_Union",
+  ``!env env1. env_rel (mk_Union lx ly) env env1 <=>
+               env_rel lx env env1 /\ env_rel ly env env1``,
+  fs [LIST_RELi_EL_EQN,env_rel_def] \\ metis_tac []);
+
+val env_rel_length = store_thm("env_rel_length",
+  ``env_rel l env env1 ==> LENGTH env1 = LENGTH env``,
+  fs [LIST_RELi_EL_EQN,env_rel_def]);
+
+val env_rel_MAPi = store_thm("env_rel_MAPi",
+  ``env_rel l1 env (MAPi (\i v. if has_var i l1 then v else Number 0) env)``,
+  fs [LIST_RELi_EL_EQN,env_rel_def]);
+
+val IMP_EL_SING = store_thm("IMP_EL_SING",
+  ``k = LENGTH xs ==> EL k (xs ++ [x] ++ ys) = x``,
+  rw [] \\ fs [] \\ full_simp_tac std_ss [GSYM APPEND_ASSOC,APPEND]
+  \\ fs [EL_APPEND2]);
+
+val ALOOKUP_MAPi_SWAP = store_thm("ALOOKUP_MAPi_SWAP",
+  ``!z n k xs.
+      n <> k ==>
+      ALOOKUP (MAPi (λi x. (x,i+z)) (xs ++ [k])) n =
+      ALOOKUP (MAPi (λi x. (x,i+z)) xs) n``,
+  Induct_on `xs` \\ fs [o_DEF,ADD1]) |> Q.SPEC `0` |> SIMP_RULE std_ss [];
+
+val ALOOKUP_MAPi_APPEND2 = store_thm("ALOOKUP_MAPi_APPEND2",
+  ``!z xs k.
+      ~MEM k xs ==>
+      ALOOKUP (MAPi (λi x. (x,i+z)) (xs ++ [k])) k = SOME (LENGTH xs + z)``,
+  Induct_on `xs` \\ fs [o_DEF,ADD1]) |> Q.SPEC `0` |> SIMP_RULE std_ss [];
+
+val evaluate_LetLet = store_thm("evaluate_LetLet",
+  ``(∀env2 extra.
+       env_rel l1 env env2 ==> evaluate ([y],env2 ++ extra,s1) = res) /\
+    env_rel l1 env env1 ==>
+    evaluate ([LetLet (LENGTH env) l1 y],env1 ++ extra,s1) = res``,
+  fs [LetLet_def] \\ rw [o_DEF] \\ fs [Once evaluate_def]
+  \\ qabbrev_tac `qs = (FILTER (λn. has_var n l1) (GENLIST I (LENGTH env)))`
+  \\ `evaluate
+        (MAP Var qs,env1 ++ extra,s1) =
+        (Rval (MAP (\i. EL i env) qs), s1)` by
+   (`EVERY (\n. has_var n l1 /\ n < LENGTH env) qs` by
+      (fs [EVERY_MEM] \\ unabbrev_all_tac \\ fs [MEM_FILTER,MEM_GENLIST])
+    \\ ntac 2 (pop_assum mp_tac \\ pop_assum kall_tac)
+    \\ Induct_on `qs` \\ fs [evaluate_def]
+    \\ once_rewrite_tac [evaluate_CONS]
+    \\ rw [] \\ fs [evaluate_def]
+    \\ imp_res_tac env_rel_length \\ fs [EL_APPEND1]
+    \\ fs [env_rel_def,LIST_RELi_EL_EQN])
+  \\ fs [evaluate_def]
+  \\ qpat_abbrev_tac `ev = bvlSem$evaluate _`
+  \\ qsuff_tac `ev =
+       (Rval (MAPi (\i v. if has_var i l1 then v else Number 0) env),s1)`
+  THEN1
+   (fs [] \\ full_simp_tac bool_ss [GSYM APPEND_ASSOC] \\ strip_tac
+    \\ first_x_assum match_mp_tac \\ fs [env_rel_MAPi])
+  \\ unabbrev_all_tac \\ rpt (pop_assum kall_tac)
+  \\ full_simp_tac bool_ss [GSYM APPEND_ASSOC]
+  \\ qspec_tac (`env1 ++ extra`,`ex`)
+  \\ qspec_tac (`env`,`env`)
+  \\ HO_MATCH_MP_TAC SNOC_INDUCT \\ rw [] \\ fs [evaluate_def]
+  \\ fs [GENLIST,SNOC_APPEND,FILTER,FILTER_APPEND]
+  \\ fs [REWRITE_RULE [SNOC_APPEND] evaluate_SNOC,MAP_APPEND]
+  \\ qpat_abbrev_tac `ev = bvlSem$evaluate _`
+  \\ `ev = (Rval (MAPi (λi v. if has_var i l1 then v else Number 0) env),s1)` by
+   (unabbrev_all_tac
+    \\ pop_assum (qspec_then `MAP (λi. EL i (env ++ [x]))
+         (if has_var (LENGTH env) l1 then [LENGTH env] else []) ++ ex` mp_tac)
+    \\ disch_then (fn th => fs [GSYM th])
+    \\ AP_TERM_TAC \\ fs [GENLIST_FUN_EQ] \\ rw []
+    THEN1
+     (ntac 3 (AP_TERM_TAC ORELSE AP_THM_TAC)
+      \\ match_mp_tac ALOOKUP_MAPi_SWAP \\ fs [])
+    \\ fs [MAP_EQ_f,MEM_FILTER,MEM_GENLIST,EL_APPEND1] \\ NO_TAC) \\ fs []
+  \\ `ALOOKUP
+        (MAPi (λi x. (x,i))
+          (FILTER (λn. has_var n l1) (GENLIST I (LENGTH env)) ++
+           if has_var (LENGTH env) l1 then [LENGTH env] else []))
+        (LENGTH env) =
+      if has_var (LENGTH env) l1 then
+        SOME (LENGTH (FILTER (λn. has_var n l1) (GENLIST I (LENGTH env))))
+      else NONE` by
+   (IF_CASES_TAC \\ fs []
+    \\ TRY (match_mp_tac ALOOKUP_MAPi_APPEND2)
+    \\ fs [MEM_FILTER,MEM_GENLIST,ALOOKUP_NONE,o_DEF,MAPi_ID] \\ NO_TAC)
+  \\ fs [] \\ reverse (Cases_on `has_var (LENGTH env) l1`) \\ fs []
+  \\ fs [evaluate_def,do_app_def,MAPi_def,MAPi_APPEND]
+  \\ fs [EL_APPEND2] \\ match_mp_tac IMP_EL_SING \\ fs []);
+
+val env_rel_refl = store_thm("env_rel_refl",
+  ``env_rel l env env``,
+  fs [LIST_RELi_EL_EQN,env_rel_def]);
+
+val compile_correct = store_thm("compile_correct",
+  ``!xs env s1 ys env1 res s2 extra l s.
+      compile (LENGTH env) xs = (ys,l,s) /\ env_rel l env env1 /\
+      (evaluate (xs,env,s1) = (res,s2)) /\ res <> Rerr(Rabort Rtype_error) ==>
+      (evaluate (ys,env1 ++ extra,s1) = (res,s2))``,
   SIMP_TAC std_ss [Once EQ_SYM_EQ]
   \\ recInduct evaluate_ind \\ REPEAT STRIP_TAC
-  \\ FULL_SIMP_TAC std_ss [compile_def,evaluate_def,compile_HD_SING]
+  \\ FULL_SIMP_TAC std_ss [compile_def,evaluate_def]
+  \\ fs [LET_THM] \\ rpt (pairarg_tac \\ fs []) \\ rveq \\ fs [env_rel_mk_Union]
+  \\ imp_res_tac compile_sing \\ rveq
+  \\ imp_res_tac env_rel_length
   THEN1 (* Cons *)
-   (ONCE_REWRITE_TAC [GSYM compile_HD_SING] \\ fs []
-    \\ SIMP_TAC std_ss [Once evaluate_CONS]
-    \\ fs [compile_HD_SING]
-    \\ Cases_on `evaluate ([x],env,s)` \\ Cases_on `q` \\ fs []
+   (Cases_on `evaluate ([x],env,s)` \\ Cases_on `q` \\ fs []
     \\ Cases_on `evaluate (y::xs,env,r)` \\ Cases_on `q` \\ fs []
-    \\ rw[] \\ fs[])
+    \\ rw[] \\ fs[] \\ res_tac \\ fs []
+    \\ SIMP_TAC std_ss [Once evaluate_CONS] \\ fs [])
   THEN1 (* Var *)
-   (Cases_on `n < LENGTH env` \\ fs []
-    \\ `n < LENGTH env + LENGTH ys` by DECIDE_TAC
-    \\ fs [compile_def,evaluate_def,rich_listTheory.EL_APPEND1])
+   (Cases_on `n < LENGTH env` \\ fs [] \\ rveq
+    \\ `n < LENGTH env1 + LENGTH extra` by DECIDE_TAC
+    \\ fs [evaluate_def,rich_listTheory.EL_APPEND1]
+    \\ fs [env_rel_def,LIST_RELi_EL_EQN])
   THEN1 (* If *)
    (Cases_on `evaluate ([x1],env,s)` \\ Cases_on `q` \\ fs []
     \\ SRW_TAC [] [] \\ fs []
-    \\ FIRST_X_ASSUM MATCH_MP_TAC \\ METIS_TAC [])
+    \\ Cases_on `Boolv T = HD a` \\ fs [] \\ res_tac \\ fs [evaluate_def]
+    \\ Cases_on `Boolv F = HD a` \\ fs [] \\ res_tac \\ fs [evaluate_def])
   THEN1 (* Let *)
-   (Cases_on `evaluate (xs,env,s)` \\ Cases_on `q` \\ fs []
-    \\ rw[] \\ fs[]
-    \\ ONCE_REWRITE_TAC [ADD_COMM]
-    \\ `LENGTH xs = LENGTH a` by (IMP_RES_TAC evaluate_IMP_LENGTH \\ fs [])
-    \\ fs [] \\ FIRST_X_ASSUM MATCH_MP_TAC \\ METIS_TAC [])
+   (Cases_on `LENGTH xs = 0` \\ fs [LENGTH_NIL] \\ rveq
+    \\ fs [evaluate_def,env_rel_mk_Union]
+    \\ Cases_on `evaluate (xs,env,s)` \\ Cases_on `q` \\ fs [] \\ rw []
+    \\ imp_res_tac evaluate_IMP_LENGTH \\ fs []
+    \\ `env_rel l2 (a ++ env) (a ++ env1)` by
+     (fs [env_rel_def,LIST_RELi_EL_EQN] \\ rw []
+      \\ Cases_on `i < LENGTH a` \\ fs [EL_APPEND1,NOT_LESS,EL_APPEND2])
+    \\ res_tac \\ fs [])
   THEN1 (* Raise *)
-   (Cases_on `evaluate ([x1],env,s)` \\ Cases_on `q` \\ fs [] \\ rw[] \\ fs[])
+   (Cases_on `evaluate ([x1],env,s)` \\ Cases_on `q` \\ fs [] \\ rw []
+    \\ res_tac \\ fs [evaluate_def])
   THEN1 (* Handle *)
-   (fs [LET_DEF,evaluate_def,compile_HD_SING,evaluate_GENLIST]
-    \\ Cases_on `evaluate ([x1],env,s1)` \\ fs []
+   (Cases_on `evaluate ([x1],env,s1)` \\ fs []
     \\ `q <> Rerr(Rabort Rtype_error)` by (REPEAT STRIP_TAC \\ fs []) \\ fs []
     \\ FULL_SIMP_TAC std_ss [GSYM APPEND_ASSOC] \\ fs []
-    \\ Cases_on `q` \\ fs [ADD1]
-    \\ Cases_on`e` \\ fs[]
-    \\ FIRST_X_ASSUM MATCH_MP_TAC \\ METIS_TAC [])
+    \\ rename1 `compile (LENGTH env) [x1] = ([yy],l1,s3)`
+    \\ Cases_on `no_raise [yy]` \\ fs [] \\ rveq \\ res_tac THEN1
+     (pop_assum (assume_tac o SPEC_ALL)
+      \\ imp_res_tac no_raise_evaluate
+      \\ every_case_tac \\ fs [])
+    \\ fs [evaluate_def,env_rel_mk_Union]
+    \\ drule evaluate_LetLet \\ fs []
+    \\ every_case_tac \\ fs [ADD1] \\ rw [] \\ rfs[]
+    \\ `env_rel l2 (a::env) (a::env1)` by
+     (fs [env_rel_def,LIST_RELi_EL_EQN]
+      \\ Cases \\ fs [ADD1]) \\ res_tac \\ fs [])
   THEN1 (* Op *)
-   (Cases_on `evaluate (xs,env,s)` \\ Cases_on `q` \\ fs [] \\ rw[] \\ fs[])
+   (Cases_on `evaluate (xs,env,s)` \\ Cases_on `q` \\ fs [] \\ rw []
+    \\ res_tac \\ fs [evaluate_def])
   THEN1 (* Tick *)
-   (Cases_on `s.clock = 0` \\ fs [compile_HD_SING]
-    \\ FIRST_X_ASSUM MATCH_MP_TAC \\ METIS_TAC [])
+   (Cases_on `s.clock = 0` \\ fs [] \\ rw [evaluate_def])
   THEN1 (* Call *)
-   (Cases_on `evaluate (xs,env,s1)` \\ Cases_on `q` \\ fs [] \\ rw[] \\ fs[]))
-  |> Q.SPECL [`xs`,`env`,`s1`,`res`,`s2`,`[]`]
-  |> SIMP_RULE std_ss [APPEND_NIL];
+   (Cases_on `evaluate (xs,env,s1)` \\ Cases_on `q` \\ fs [] \\ rw[]
+    \\ every_case_tac \\ fs [evaluate_def]))
+  |> Q.SPECL [`xs`,`env`,`s1`,`ys`,`env`,`res`,`s2`,`[]`]
+  |> SIMP_RULE std_ss [APPEND_NIL,env_rel_refl];
 
 val _ = save_thm("compile_correct",compile_correct);
 
-val bVarBound_compile = Q.store_thm("bVarBound_compile",
-  `∀n xs m. n ≤ m ⇒ bVarBound m (compile n xs)`,
-  ho_match_mp_tac compile_ind >>
-  rw[compile_def,bVarBound_def,compile_HD_SING,LET_THM] >>
-  fs[Once bVarBound_EVERY,EVERY_GENLIST] >> simp[]);
+val compile_correct = store_thm("compile_correct",
+  ``(evaluate ([x],env,s1) = (res,s2)) /\ res <> Rerr(Rabort Rtype_error) /\
+    k = LENGTH env ==>
+    (evaluate ([compile_exp k x],env,s1) = (res,s2))``,
+  fs [compile_exp_def]
+  \\ Cases_on `compile (LENGTH env) [x]` \\ PairCases_on `r`
+  \\ rw [] \\ imp_res_tac compile_sing \\ rw []
+  \\ imp_res_tac compile_correct);
 
-val compile_GoodHandleLet = Q.store_thm("compile_GoodHandleLet",
-  `∀n xs. bEvery GoodHandleLet (compile n xs)`,
-  ho_match_mp_tac compile_ind >>
-  rw[compile_def,compile_HD_SING,LET_THM] >>
-  fs[EVERY_GENLIST,isVar_def,Once bEvery_EVERY] >>
-  match_mp_tac bVarBound_compile >> simp[]);
+val compile_IMP_LENGTH = store_thm("compile_IMP_LENGTH",
+  ``compile n xs = (ys,l1,s1) ==> LENGTH ys = LENGTH xs``,
+  rw [] \\ mp_tac (SPEC_ALL compile_length) \\ asm_simp_tac std_ss []);
+
+val bVarBound_CONS = store_thm("bVarBound_CONS",
+  ``bVarBound m [x] /\ bVarBound m xs ==> bVarBound m (x::xs)``,
+  Cases_on `xs` \\ fs []);
+
+val bVarBound_MEM = store_thm("bVarBound_MEM",
+  ``bVarBound n xs <=> !x. MEM x xs ==> bVarBound n [x]``,
+  fs [Once bVarBound_EVERY,EVERY_MEM]);
+
+val bEvery_MEM = store_thm("bEvery_MEM",
+  ``bEvery p xs = !x. MEM x xs ==> bEvery p [x]``,
+  fs [Once bEvery_EVERY,EVERY_MEM]);
+
+val bVarBound_LESS_EQ = store_thm("bVarBound_LESS_EQ",
+  ``!m xs n. bVarBound m xs /\ m <= n ==> bVarBound n xs``,
+  HO_MATCH_MP_TAC bVarBound_ind \\ rw [] \\ fs []);
+
+val ALOOKUP_MAPi = store_thm("ALOOKUP_MAPi",
+  ``!xs i x.
+      ALOOKUP (MAPi (λi x. (x,i)) xs) n = SOME x ==> x < LENGTH xs``,
+  HO_MATCH_MP_TAC SNOC_INDUCT \\ rw []
+  \\ fs [SNOC_APPEND,MAPi_APPEND,ALOOKUP_APPEND]
+  \\ every_case_tac \\ fs []);
+
+val bVarBound_LetLet = store_thm("bVarBound_LetLet",
+  ``bVarBound m [y] /\ n <= m ==> bVarBound m [LetLet n l1 y]``,
+  fs [LetLet_def] \\ strip_tac
+  \\ once_rewrite_tac [bVarBound_MEM]
+  \\ fs [MEM_MAP,MEM_GENLIST,PULL_EXISTS,MEM_FILTER]
+  \\ reverse conj_tac
+  THEN1 (match_mp_tac bVarBound_LESS_EQ \\ asm_exists_tac \\ fs [])
+  \\ rw [] \\ every_case_tac \\ fs []
+  \\ qabbrev_tac `xs = FILTER (λn. has_var n l1) (GENLIST I n)`
+  \\ imp_res_tac ALOOKUP_MAPi \\ fs []);
+
+val bVarBound_compile = Q.store_thm("bVarBound_compile",
+  `∀n xs m. n ≤ m ⇒ bVarBound m (FST (compile n xs))`,
+  ho_match_mp_tac compile_ind \\ rw [] \\ fs [compile_def]
+  \\ rpt (pairarg_tac \\ fs []) \\ rveq
+  \\ imp_res_tac compile_sing \\ rw [] \\ res_tac
+  \\ imp_res_tac bVarBound_CONS \\ fs []
+  \\ TRY (first_x_assum match_mp_tac) \\ fs []
+  \\ imp_res_tac compile_IMP_LENGTH \\ fs []
+  \\ imp_res_tac bVarBound_LetLet \\ fs []);
+
+val bEvery_CONS = store_thm("bEvery_CONS",
+  ``bEvery p [x] /\ bEvery p xs ==> bEvery p (x::xs)``,
+  Cases_on `xs` \\ fs []);
+
+val compile_GoodHandleLet = store_thm("compile_GoodHandleLet",
+  ``∀n xs. bEvery GoodHandleLet (FST (compile n xs))``,
+  ho_match_mp_tac compile_ind \\ rw [] \\ fs [compile_def]
+  \\ rpt (pairarg_tac \\ fs []) \\ rveq
+  \\ imp_res_tac compile_sing \\ rw [] \\ res_tac
+  \\ imp_res_tac bEvery_CONS \\ fs []
+  THEN1
+   (fs [GoodHandleLet_def,LetLet_def,EVERY_MEM,MEM_MAP,PULL_EXISTS,isVar_def]
+    \\ reverse conj_tac THEN1
+     (`[y'] = FST (compile n [x1])` by fs []
+      \\ pop_assum (fn th => rewrite_tac [th])
+      \\ match_mp_tac bVarBound_compile \\ fs [])
+    \\ once_rewrite_tac [bVarBound_MEM]
+    \\ fs [MEM_GENLIST,PULL_EXISTS] \\ rw []
+    \\ every_case_tac \\ fs []
+    \\ imp_res_tac ALOOKUP_MAPi \\ fs [])
+  \\ fs [LetLet_def]
+  \\ once_rewrite_tac [bEvery_MEM]
+  \\ fs [MEM_GENLIST,PULL_EXISTS,MEM_MAP] \\ rw []
+  \\ every_case_tac \\ fs []);
+
+val compile_exp_GoodHandleLet = store_thm("compile_exp_GoodHandleLet",
+  ``bEvery GoodHandleLet [compile_exp n x]``,
+  fs [bvl_handleTheory.compile_exp_def]
+  \\ Cases_on `compile n [x]` \\ fs [] \\ PairCases_on `r`
+  \\ imp_res_tac bvl_handleTheory.compile_sing \\ fs []
+  \\ qspecl_then [`n`,`[x]`] mp_tac compile_GoodHandleLet \\ fs []);
 
 val _ = export_theory();
